src/ocaml/extraction/Options0.mli
@@ -4,4 +4,5 @@ type options = { add_carry_constraints : bool;
                  rewrite_assignments_imp : bool;
                  vars_cache_in_rewrite_assignments : bool;
                  compute_coefficients_one_by_one : bool;
-                 apply_slicing_espec : bool; apply_slicing_rspec : bool }
+                 apply_slicing_espec : bool; apply_slicing_rspec : bool;
+                 apply_slicing_assume : bool }
