src/ocaml/extraction/SSA2ZSSA.ml
@@ -53,8 +53,8 @@ let algred_is_carry c =
 
 (** val carry_constr : options -> ssavar -> SSA.SSA.ebexp list **)
 
-let carry_constr options0 c =
-  if options0.add_carry_constraints then (algred_is_carry c) :: [] else []
+let carry_constr o c =
+  if o.add_carry_constraints then (algred_is_carry c) :: [] else []
 
 (** val algred_cast :
     VarOrder.t -> coq_N -> SSAVarOrder.t -> typ -> SSA.SSA.atom -> typ ->
@@ -109,7 +109,7 @@ let algred_vpc _ g v a =
     options -> TypEnv.SSATE.env -> VarOrder.t -> coq_N -> SSA.SSA.instr ->
     coq_N * SSA.SSA.ebexp list **)
 
-let algred_instr options0 te avn g = function
+let algred_instr o te avn g = function
 | SSA.SSA.Imov (v, a) ->
   let za = algred_atom a in (g, ((algred_assign v za) :: []))
 | SSA.SSA.Ishl (v, a, n) ->
@@ -125,7 +125,7 @@ let algred_instr options0 te avn g = function
      (subn a2size n)) :: []))
 | SSA.SSA.Inondet (v, t0) ->
   if eq_op typ_eqType (Obj.magic t0) (Obj.magic coq_Tbit)
-  then (g, (carry_constr options0 v))
+  then (g, (carry_constr o v))
   else (g, [])
 | SSA.SSA.Icmov (v, c, a1, a2) ->
   let zc = algred_atom c in
@@ -166,7 +166,7 @@ let algred_instr options0 te avn g = function
    | Tuint w ->
      (g,
        (cat ((algred_split c v (SSA.SSA.eadd za1 za2) w) :: [])
-         (carry_constr options0 c)))
+         (carry_constr o c)))
    | Tsint _ -> (g, ((algred_assign v (SSA.SSA.eadd za1 za2)) :: [])))
 | SSA.SSA.Iadc (v, a1, a2, y) ->
   let za1 = algred_atom a1 in
@@ -182,7 +182,7 @@ let algred_instr options0 te avn g = function
      (g,
        (cat
          ((algred_split c v (SSA.SSA.eadd (SSA.SSA.eadd za1 za2) zy) w) :: [])
-         (carry_constr options0 c)))
+         (carry_constr o c)))
    | Tsint _ ->
      (g, ((algred_assign v (SSA.SSA.eadd (SSA.SSA.eadd za1 za2) zy)) :: [])))
 | SSA.SSA.Isub (v, a1, a2) ->
@@ -198,7 +198,7 @@ let algred_instr options0 te avn g = function
        (cat
          ((algred_join (SSA.SSA.evar v)
             (SSA.SSA.esub (SSA.SSA.econst Z.one) (SSA.SSA.evar c))
-            (SSA.SSA.esub za1 za2) w) :: []) (carry_constr options0 c)))
+            (SSA.SSA.esub za1 za2) w) :: []) (carry_constr o c)))
    | Tsint _ -> (g, ((algred_assign v (SSA.SSA.esub za1 za2)) :: [])))
 | SSA.SSA.Isubb (c, v, a1, a2) ->
   let za1 = algred_atom a1 in
@@ -208,7 +208,7 @@ let algred_instr options0 te avn g = function
      (g,
        (cat
          ((algred_join (SSA.SSA.evar v) (SSA.SSA.evar c)
-            (SSA.SSA.esub za1 za2) w) :: []) (carry_constr options0 c)))
+            (SSA.SSA.esub za1 za2) w) :: []) (carry_constr o c)))
    | Tsint _ -> (g, ((algred_assign v (SSA.SSA.esub za1 za2)) :: [])))
 | SSA.SSA.Isbc (v, a1, a2, y) ->
   let za1 = algred_atom a1 in
@@ -230,7 +230,7 @@ let algred_instr options0 te avn g = function
             (SSA.SSA.esub (SSA.SSA.econst Z.one) (SSA.SSA.evar c))
             (SSA.SSA.esub (SSA.SSA.esub za1 za2)
               (SSA.SSA.esub (SSA.SSA.econst Z.one) zy)) w) :: [])
-         (carry_constr options0 c)))
+         (carry_constr o c)))
    | Tsint _ ->
      (g,
        ((algred_assign v
@@ -251,7 +251,7 @@ let algred_instr options0 te avn g = function
        (cat
          ((algred_join (SSA.SSA.esub (SSA.SSA.esub za1 za2) zy)
             (SSA.SSA.eneg (SSA.SSA.evar c)) (SSA.SSA.evar v) w) :: [])
-         (carry_constr options0 c)))
+         (carry_constr o c)))
    | Tsint _ ->
      (g, ((algred_assign v (SSA.SSA.esub (SSA.SSA.esub za1 za2) zy)) :: [])))
 | SSA.SSA.Imul (v, a1, a2) ->
@@ -283,12 +283,12 @@ let algred_instr options0 te avn g = function
     options -> TypEnv.SSATE.env -> VarOrder.t -> coq_N -> SSA.SSA.program ->
     coq_N * SSA.SSA.ebexp list **)
 
-let rec algred_program options0 te avn g = function
+let rec algred_program o te avn g = function
 | [] -> (g, [])
 | hd :: tl ->
-  let (g_hd, zhd) = algred_instr options0 te avn g hd in
+  let (g_hd, zhd) = algred_instr o te avn g hd in
   let (g_tl, ztl) =
-    algred_program options0 (SSA.SSA.instr_succ_typenv hd te) avn g_hd tl
+    algred_program o (SSA.SSA.instr_succ_typenv hd te) avn g_hd tl
   in
   (g_tl, (cat zhd ztl))
 
@@ -304,9 +304,9 @@ let new_svar_spec s =
 (** val algred_espec :
     options -> VarOrder.t -> SSA.SSA.espec -> ZSSA.ZSSA.rep **)
 
-let algred_espec options0 avn s =
+let algred_espec o avn s =
   let (_, eprogs) =
-    algred_program options0 (SSA.SSA.esinputs s) avn SSA.initial_index
+    algred_program o (SSA.SSA.esinputs s) avn SSA.initial_index
       (SSA.SSA.esprog s)
   in
   { ZSSA.ZSSA.premise =
