src/ocaml/options/std.mli
@@ -53,6 +53,7 @@ val apply_rewriting_imp : bool ref
 val polys_rewrite_replace_eexp : bool ref
 val apply_slicing_espec : bool ref
 val apply_slicing_rspec : bool ref
+val apply_slicing_assume : bool ref
 
 val variable_ordering : variable_order ref
 val string_of_variable_ordering : variable_order -> string
